

# Introduction to Artificial Intelligence with Python

Dr.Bayan O. Mohammed  
2024-2025

# Inference Rules

# Modus Ponens

If it is raining, then Harry is inside.

It is raining.

---

Harry is inside.

# Modus Ponens

$$\alpha \rightarrow \beta$$

$$\alpha$$



$$\beta$$

# And Elimination

Harry is friends with Ron and Hermione.

---

Harry is friends with Hermione.

# And Elimination

$$\alpha \wedge \beta$$

---

$$\alpha$$

# Double Negation Elimination

It is not true that Harry did not pass the test.

---

Harry passed the test.

# Double Negation Elimination

$$\neg(\neg\alpha)$$

---

$$\alpha$$



# Implication Elimination

If it is raining, then Harry is inside.

---

It is not raining or Harry is inside.

# Implication Elimination

$$\alpha \rightarrow \beta$$



$$\neg \alpha \vee \beta$$

# Biconditional Elimination

It is raining if and only if Harry is inside.

---

If it is raining, then Harry is inside,  
and if Harry is inside, then it is raining.

# Biconditional Elimination

$$\alpha \leftrightarrow \beta$$

---

$$(\alpha \rightarrow \beta) \wedge (\beta \rightarrow \alpha)$$

# De Morgan's Law

It is not true that both  
Harry and Ron passed the test.

---

Harry did not pass the test  
or Ron did not pass the test.

# De Morgan's Law

$$\neg(a \wedge \beta)$$

---

$$\neg a \vee \neg \beta$$

# De Morgan's Law

It is not true that  
Harry or Ron passed the test.

---

Harry did not pass the test  
and Ron did not pass the test.

# De Morgan's Law

$$\neg(a \vee \beta)$$

---

$$\neg a \wedge \neg \beta$$



# Distributive Property

$$(a \wedge (\beta \vee \gamma))$$

---

$$(a \wedge \beta) \vee (a \wedge \gamma)$$

# Distributive Property

$$(a \vee (\beta \wedge \gamma))$$

---

$$(a \vee \beta) \wedge (a \vee \gamma)$$

# Search Problems

- initial state
- actions
- transition model
- goal test
- path cost function

# Theorem Proving

- initial state: starting knowledge base
- actions: inference rules
- transition model: new knowledge base after inference
- goal test: check statement we're trying to prove
- path cost function: number of steps in proof

# Resolution

$(\text{Ron is in the Great Hall}) \vee (\text{Hermione is in the library})$

Ron is not in the Great Hall

---

Hermione is in the library

$$P \vee Q$$

$$\neg P$$

---

$$Q$$

$$P \vee Q_1 \vee Q_2 \vee \dots \vee Q_n$$

$$\neg P$$

---


$$Q_1 \vee Q_2 \vee \dots \vee Q_n$$



$(\text{Ron is in the Great Hall}) \vee (\text{Hermione is in the library})$

$(\text{Ron is not in the Great Hall}) \vee (\text{Harry is sleeping})$

---

$(\text{Hermione is in the library}) \vee (\text{Harry is sleeping})$

$$P \vee Q$$

$$\neg P \vee R$$

---

$$Q \vee R$$

$$P \vee Q_1 \vee Q_2 \vee \dots \vee Q_n$$

$$\neg P \vee R_1 \vee R_2 \vee \dots \vee R_m$$

---


$$Q_1 \vee Q_2 \vee \dots \vee Q_n \vee R_1 \vee R_2 \vee \dots \vee R_m$$

# clause

a disjunction of literals

e.g.  $P \vee Q \vee R$

# conjunctive normal form

logical sentence that is a conjunction of clauses

e.g.  $(A \vee B \vee C) \wedge (D \vee \neg E) \wedge (F \vee G)$

# Conversion to CNF

- Eliminate biconditionals
  - turn  $(\alpha \leftrightarrow \beta)$  into  $(\alpha \rightarrow \beta) \wedge (\beta \rightarrow \alpha)$
- Eliminate implications
  - turn  $(\alpha \rightarrow \beta)$  into  $\neg\alpha \vee \beta$
- Move  $\neg$  inwards using De Morgan's Laws
  - e.g. turn  $\neg(\alpha \wedge \beta)$  into  $\neg\alpha \vee \neg\beta$
- Use distributive law to distribute  $\vee$  wherever possible

# Conversion to CNF

$$(P \vee Q) \rightarrow R$$

$$\neg(P \vee Q) \vee R$$

eliminate implication

$$(\neg P \wedge \neg Q) \vee R$$

De Morgan's Law

$$(\neg P \vee R) \wedge (\neg Q \vee R)$$

distributive law

# Inference by Resolution



$$P \vee Q$$

$$\neg P \vee R$$

---

$$(Q \vee R)$$

$$P \vee Q \vee S$$

$$\neg P \vee R \vee S$$

---

$$(Q \vee S \vee R \vee S)$$

$$P \vee Q \vee S$$

$$\neg P \vee R \vee S$$

---


$$(Q \vee R \vee S)$$

$P$

$\neg P$



$()$

# Inference by Resolution

- To determine if  $KB \models \alpha$ :
  - Check if  $(KB \wedge \neg \alpha)$  is a contradiction?
    - If so, then  $KB \models \alpha$ .
    - Otherwise, no entailment.

# Inference by Resolution

- To determine if  $KB \models \alpha$ :
  - Convert  $(KB \wedge \neg\alpha)$  to Conjunctive Normal Form.
  - Keep checking to see if we can use resolution to produce a new clause.
    - If ever we produce the **empty** clause (equivalent to False), we have a contradiction, and  $KB \models \alpha$ .
    - Otherwise, if we can't add new clauses, no entailment.

# Inference by Resolution

Does  $(A \vee B) \wedge (\neg B \vee C) \wedge (\neg C)$  entail  $A$ ?

$$(A \vee B) \wedge (\neg B \vee C) \wedge (\neg C) \wedge (\neg A)$$

$$(A \vee B) \quad (\neg B \vee C) \quad (\neg C) \quad (\neg A)$$

# Inference by Resolution

Does  $(A \vee B) \wedge (\neg B \vee C) \wedge (\neg C)$  entail  $A$ ?

$$(A \vee B) \wedge (\neg B \vee C) \wedge (\neg C) \wedge (\neg A)$$

$$(A \vee B) \quad \underline{(\neg B \vee C)} \quad \underline{(\neg C)} \quad (\neg A)$$



# Inference by Resolution

Does  $(A \vee B) \wedge (\neg B \vee C) \wedge (\neg C)$  entail  $A$ ?

$$(A \vee B) \wedge (\neg B \vee C) \wedge (\neg C) \wedge (\neg A)$$

$$(A \vee B) \quad \underline{(\neg B \vee C)} \quad \underline{(\neg C)} \quad (\neg A) \quad (\neg B)$$

# Inference by Resolution

Does  $(A \vee B) \wedge (\neg B \vee C) \wedge (\neg C)$  entail  $A$ ?

$$(A \vee B) \wedge (\neg B \vee C) \wedge (\neg C) \wedge (\neg A)$$

$$(A \vee B) \quad (\neg B \vee C) \quad (\neg C) \quad (\neg A) \quad (\neg B)$$

# Inference by Resolution

Does  $(A \vee B) \wedge (\neg B \vee C) \wedge (\neg C)$  entail  $A$ ?

$$(A \vee B) \wedge (\neg B \vee C) \wedge (\neg C) \wedge (\neg A)$$

$$\underline{(A \vee B)} \quad (\neg B \vee C) \quad (\neg C) \quad (\neg A) \quad \underline{(\neg B)}$$

# Inference by Resolution

Does  $(A \vee B) \wedge (\neg B \vee C) \wedge (\neg C)$  entail  $A$ ?

$$(A \vee B) \wedge (\neg B \vee C) \wedge (\neg C) \wedge (\neg A)$$

$$\underline{(A \vee B)} \quad (\neg B \vee C) \quad (\neg C) \quad (\neg A) \quad \underline{(\neg B)} \quad (A)$$

# Inference by Resolution

Does  $(A \vee B) \wedge (\neg B \vee C) \wedge (\neg C)$  entail  $A$ ?

$$(A \vee B) \wedge (\neg B \vee C) \wedge (\neg C) \wedge (\neg A)$$

$$(A \vee B) \quad (\neg B \vee C) \quad (\neg C) \quad (\neg A) \quad (\neg B) \quad (A)$$

# Inference by Resolution

Does  $(A \vee B) \wedge (\neg B \vee C) \wedge (\neg C)$  entail  $A$ ?

$$(A \vee B) \wedge (\neg B \vee C) \wedge (\neg C) \wedge (\neg A)$$

$$(A \vee B) \quad (\neg B \vee C) \quad (\neg C) \quad \underline{(\neg A)} \quad (\neg B) \quad \underline{(A)}$$

# Inference by Resolution

Does  $(A \vee B) \wedge (\neg B \vee C) \wedge (\neg C)$  entail  $A$ ?

$$(A \vee B) \wedge (\neg B \vee C) \wedge (\neg C) \wedge (\neg A)$$

$$(A \vee B) \quad (\neg B \vee C) \quad (\neg C) \quad \underline{(\neg A)} \quad (\neg B) \quad \underline{(A)} \quad ()$$

# Inference by Resolution

Does  $(A \vee B) \wedge (\neg B \vee C) \wedge (\neg C)$  entail  $A$ ?

$$(A \vee B) \wedge (\neg B \vee C) \wedge (\neg C) \wedge (\neg A)$$

$$(A \vee B) \quad (\neg B \vee C) \quad (\neg C) \quad (\neg A) \quad (\neg B) \quad (A) \quad ()$$



# First-Order Logic

# Propositional Logic

## Propositional Symbols

*MinervaGryffindor*

*MinervaHufflepuff*

*MinervaRavenclaw*

*MinervaSlytherin*

...

# First-Order Logic

## Constant Symbol

*Minerva*

*Pomona*

*Horace*

*Gilderoy*

*Gryffindor*

*Hufflepuff*

*Ravenclaw*

*Slytherin*

## Predicate Symbol

*Person*

*House*

*BelongsTo*

# First-Order Logic

*Person(Minerva)*

Minerva is a person.

*House(Gryffindor)*

Gryffindor is a house.

$\neg$ *House(Minerva)*

Minerva is not a house.

*BelongsTo(Minerva, Gryffindor)*

Minerva belongs to Gryffindor.

# Universal Quantification

# Universal Quantification

$$\forall x. \textit{BelongsTo}(x, \textit{Gryffindor}) \rightarrow \\ \neg \textit{BelongsTo}(x, \textit{Hufflepuff})$$

For all objects  $x$ , if  $x$  belongs to Gryffindor,  
then  $x$  does not belong to Hufflepuff.

Anyone in Gryffindor is not in Hufflepuff.

# Existential Quantification

# Existential Quantification

$$\exists x. \textit{House}(x) \wedge \textit{BelongsTo}(\textit{Minerva}, x)$$

There exists an object  $x$  such that  
 $x$  is a house and Minerva belongs to  $x$ .

Minerva belongs to a house.



# Existential Quantification

$$\forall x. \textit{Person}(x) \rightarrow (\exists y. \textit{House}(y) \wedge \textit{BelongsTo}(x, y))$$

For all objects  $x$ , if  $x$  is a person, then there exists an object  $y$  such that  $y$  is a house and  $x$  belongs to  $y$ .

Every person belongs to a house.

Knowledge

Thanks